a stable version using new idea for subsystem

theories/IsCanonical.v
@@ -1,10 +1,11 @@
-From Coq Require Import List.
 From Coq Require Import Relations.Relation_Definitions.
 From Coq Require Import Relations.Relation_Operators.
+Require Import MyRelations.
 
-Require Import Autosubst.Autosubst.
+From Autosubst Require Import Autosubst.
 Require Import LambdaM.
 
+From Coq Require Import List.
 Import ListNotations.
 
 (* ------------------------------- *)
@@ -39,14 +40,21 @@ Scheme sim_is_canonical_ind := Induction for is_canonical Sort Prop
 
 Combined Scheme mut_is_canonical_ind from sim_is_canonical_ind, sim_is_canonical_list_ind.
 
-(* definition of @ operation in λm *)
-(* ------------------------------- *)
+(* definition of h maximal reduction in in λm *)
+(* ------------------------------------------ *)
 
-Definition app (v u: term) (l: list term) : term :=
+Definition capp (v u: term) (l: list term) : term :=
   match v with
   | Var x        => mApp v u l
   | Lam t        => mApp v u l
   | mApp t u' l' => mApp t u' (l' ++ (u::l))
+  end.
+
+Fixpoint h (t: term) :=
+  match t with
+  | Var x      => Var x
+  | Lam t      => Lam (h t)
+  | mApp t u l => capp (h t) (h u) (map h l)
   end.
 
 (* lets prove that the image of h is canonical *)
@@ -60,9 +68,9 @@ Proof.
   induction l1 ; simpl ; inversion il1 ; subst ; auto.
 Qed.
 
-Lemma app_is_canonical t u l :
+Lemma capp_is_canonical t u l :
   is_canonical t -> is_canonical u -> is_canonical_list l ->
-  is_canonical (app t u l).
+  is_canonical (capp t u l).
 Proof.
   intros it iu il.
   destruct t as [x | t | v u' l'] ; asimpl ; auto.
@@ -73,15 +81,80 @@ Proof.
     + constructor ; try easy.
       * apply list_append_is_canonical ; auto.
 Qed.
-  
-(* app does H reduction *)
-(* -------------------- *)
 
-Theorem app_is_multistep_H t u l :
-  multistep_H (mApp t u l) (app t u l).
+Theorem h_is_canonical :
+  (forall t, is_canonical (h t))
+  /\
+  (forall l, is_canonical_list (map h l)).
 Proof.
-  destruct t ; asimpl ; try constructor.
-  - apply rt1n_trans with (mApp t1 t2 (l0 ++ u :: l)).
-    + now constructor.
-    + now constructor.
+  apply mut_term_ind ; intros ; asimpl ; auto.
+  - apply capp_is_canonical ; auto.
 Qed.
+
+Theorem h_is_surjective :
+  (forall t, is_canonical t -> t = h t)
+  /\
+  (forall l, is_canonical_list l -> l = map h l).
+Proof.
+  apply mut_is_canonical_ind ;
+    intros ; asimpl ; repeat f_equal ; auto.
+Qed.  
+
+(* useful lemmas relating to map h *)
+(* ------------------------------- *)
+
+Lemma capp_h_comm t u l :
+  is_canonical u ->
+  is_canonical_list l ->
+  capp (h t) u l = h (mApp t u l).
+Proof.
+  destruct t ; intros ; asimpl ; f_equal ;
+    now apply h_is_surjective.
+Qed.
+
+Lemma capp_is_multistep_H t u l :
+  multistep_H (mApp t u l) (capp t u l).
+Proof.
+  destruct t ; asimpl.
+  - apply rt1n_refl.
+  - apply rt1n_refl.
+  - apply rt1n_trans with (mApp t1 t2 (l0 ++ u :: l)).
+    + constructor. now constructor.
+    + apply rt1n_refl.
+Qed.
+
+Lemma h_is_multistep_H :
+  (forall t, multistep_H t (h t))
+  /\
+  (forall l, multistep_H' l (map h l)).
+Proof.
+  pose multistep_H_is_compatible as Hmic.
+
+  apply mut_term_ind ; intros ; asimpl ; try constructor.
+  - apply comp_lam with multistep_H' ; easy.
+  - apply multistep_trans with (mApp (h t) u l).
+    + apply comp_mApp1 with multistep_H' ; easy.
+    + apply multistep_trans with (mApp (h t) (h u) l).
+      * apply comp_mApp2 with multistep_H' ; easy.
+      * apply multistep_trans with (mApp (h t) (h u) (map h l)).
+        ** apply comp_mApp3 with multistep_H' ; easy.
+        ** apply capp_is_multistep_H.
+  - apply multistep_trans with (h u :: l).    
+    + apply comp_head with multistep_H ; easy.
+    + apply multistep_trans with (h u :: map h l).
+      * apply comp_tail with multistep_H ; easy.
+      * apply rt1n_refl.
+Qed.
+
+(* one step reduction in the canonical subsystem *)
+(* --------------------------------------------- *)
+  
+Inductive canonical_relation (R: relation term): relation term :=
+| Step_CanTerm t t' : R t t' ->
+                      canonical_relation R (h t) (h t').
+
+Inductive canonical_list_relation (R: relation (list term)): relation (list term) :=
+| Step_CanList l l' : R l l' -> canonical_list_relation R (map h l) (map h l').
+
+Definition step_can := canonical_relation step_β.
+Definition step_can' := canonical_list_relation step_β'.
